---
title: ART.T458 - Assignment - 3
UpdatedAt: Tue, 22 Jun 2021 01:13:10 +0900
---
What we want to find is the gradient of this function:

$$
J(\boldsymbol{w}) \equiv \frac{1}{n} \sum_{i=1}^{n} \ln \left(1+\exp \left(-y_{i} \boldsymbol{w}^{\top} \boldsymbol{x}_{i}\right)\right)+\lambda \boldsymbol{w}^{\top} \boldsymbol{w}
$$

Directly take the partial derivative of $w$ to get:

$$
\frac{\partial J(\boldsymbol{w})}{\partial \boldsymbol{w}}=\frac{1}{n} \sum_{i=1}^{n} \frac{\exp \left(-y_{i} \boldsymbol{w}^{\top} \boldsymbol{x}_{i}\right) \cdot\left(-y_{i} \boldsymbol{x}_{i}\right)}{1+\exp \left(-y_{i} \boldsymbol{w}^{\top} \boldsymbol{x}_{i}\right)}+2 \lambda \boldsymbol{w}
$$

Recall that the posterior probability $p(y|x)$ can be written as

$$
\begin{aligned}
p(y \mid \boldsymbol{x}) &=\frac{1}{1+\exp \left(-y \boldsymbol{w}^{\top} \boldsymbol{x}\right)}, \\
1-p(y \mid \boldsymbol{x}) &=\frac{\exp \left(-y \boldsymbol{w}^{\top} \boldsymbol{x}\right)}{1+\exp \left(-y \boldsymbol{w}^{\top} \boldsymbol{x}\right)}.
\end{aligned}
$$

The gradient can be write as 
$$
\frac{\partial J(\boldsymbol{w})}{\partial \boldsymbol{w}}=\sum_{i=1}^{n}\left(-y_{i} \boldsymbol{x}_{i}\left(1-p\left(y_{i} \mid \boldsymbol{x}_{i}\right)\right)+2 \lambda \boldsymbol{w}\right..
$$